FOL/Cardinal.thy
@@ -1,7 +1,7 @@
 (* Based on OrderType and Cardinal in Isabelle/ZF. *)
 
 theory Cardinal
-  imports Finite
+  imports Finite WellOrder
 begin
 
 section \<open>Least ordinal satisfying a property\<close>
@@ -90,7 +90,7 @@ lemma ordermap_fun_eval [rewrite]:
 setup {* del_prfstep_thm @{thm ordermap_fun_def} *}
 
 lemma ordermap_inj [forward]:
-  "wf(r) \<Longrightarrow> linorder(r) \<Longrightarrow> injective(ordermap_fun(r))"
+  "well_order(r) \<Longrightarrow> injective(ordermap_fun(r))"
 @proof
   @let "f = ordermap_fun(r)"
   @have "\<forall>x\<in>.r. \<forall>y\<in>.r. x \<noteq> y \<longrightarrow> f`x \<noteq> f`y" @with
@@ -104,7 +104,7 @@ lemma ordermap_inj [forward]:
 @qed
 
 lemma ordermap_bij [forward]:
-  "wf(r) \<Longrightarrow> linorder(r) \<Longrightarrow> bijective(ordermap_fun(r))"
+  "well_order(r) \<Longrightarrow> bijective(ordermap_fun(r))"
   by auto2
 
 section \<open>Cardinals\<close>
@@ -117,8 +117,9 @@ definition card :: "i \<Rightarrow> o" where [rewrite]:
 
 section \<open>Basic properties of cardinals\<close>
 
-lemma cardinal_equipotent [resolve]:
-  "wf(r) \<Longrightarrow> linorder(r) \<Longrightarrow> A = carrier(r) \<Longrightarrow> equipotent(A,cardinal(A))"
+(* Without assuming axiom of choice *)
+lemma cardinal_equipotent_gen [resolve]:
+  "well_order(r) \<Longrightarrow> A = carrier(r) \<Longrightarrow> equipotent(A,cardinal(A))"
 @proof
   @let "i = ordertype(r)"
   @have "equipotent(A,i)" @with
@@ -126,13 +127,26 @@ lemma cardinal_equipotent [resolve]:
   @end
 @qed
 
-lemma card_is_ordinal:
-  "wf(r) \<Longrightarrow> linorder(r) \<Longrightarrow> A = carrier(r) \<Longrightarrow> ord(cardinal(A))"
+lemma card_is_ordinal_gen [forward]:
+  "well_order(r) \<Longrightarrow> A = carrier(r) \<Longrightarrow> ord(cardinal(A))"
 @proof
   @let "i = ordertype(r)"
   @have "equipotent(A,i)" @with
     @have "ordermap_fun(r) \<in> A \<cong> ordertype(r)"
   @end
+@qed
+
+(* With axiom of choice. Will make this assumption from now on. *)
+lemma cardinal_equipotent [resolve]:
+  "equipotent(A,cardinal(A))"
+@proof
+  @obtain "R\<in>raworder_space(A)" where "well_order(R)"
+@qed
+
+lemma card_is_ordinal [forward]:
+  "ord(cardinal(A))"
+@proof
+  @obtain "R\<in>raworder_space(A)" where "well_order(R)"
 @qed
 
 end
